1) fixed redundant checks in wf_gvar 2) proved the WF-preservation for fdef-prod-module-system in top_wfS.v 3) top_wfS also proved that passes that preserve the function signatures in context should preserve WF of all components. The property should be also reused by all other passes of mem2reg. 4) proved that phiplacement preserves promotability 5) solved all admitted lemmas in phiplacement_bsim_defs.v except the typing issues in r3962 +
  there are two functions that compute CFGs in the type-checker. Rather
than proving they are the same, we should remove one of them.
6) hoisted some anonymous functions in mem2reg.v to top to simplify proofs.



git-svn-id: https://webdav.seas.upenn.edu/svn/sol/vol@3964 eef5ea85-cc2e-0410-bd84-0fae1f012da8

src3.0/Transforms/dtree.v
@@ -62,12 +62,6 @@ Qed.
 
 End MoreMove.
 
-Definition getEntryLabel (f:fdef) : option l :=
-match f with
-| fdef_intro _ ((block_intro l0 _ _ _)::_) => Some l0
-| _ => None
-end.
-
 Program Fixpoint reachablity_analysis_aux (nvisited: list l) (succs : ATree.t ls)
   (curr: l) (acc: list l) {measure (List.length nvisited)%nat}
   : option (list l) :=
